euclid gcd example

DenotationalLean/CDeriv.lean
@@ -4,13 +4,15 @@ import DenotationalLean.ADeriv
 import DenotationalLean.BDeriv
 import DenotationalLean.State
 
+import Mathlib.Tactic
+
 /-! # 2.4 The execution of commands -/
 
 abbrev CConfig := Com × State
 
 inductive c_deriv : CConfig -> State -> Prop
   | skip {σ} : c_deriv (Com.Skip, σ) σ
-  | assign {a n l σ} : a_deriv (a, σ) n -> c_deriv (Com.Assing l a, σ) ((l,n)::σ)
+  | assign {a n l σ} : a_deriv (a, σ) n -> c_deriv (Com.Assign l a, σ) ((l,n)::σ)
   | seq {c0 c1 σ σ' σ''} : c_deriv (c0,σ) σ'' -> c_deriv (c1,σ'') σ' -> c_deriv (Com.Seq c0 c1, σ) σ'
   | ite_true  {b c0 c1 σ σ'} : b_deriv (b,σ) true  -> c_deriv (c0,σ) σ' -> c_deriv (Com.Ite b c0 c1, σ) σ'
   | ite_false {b c0 c1 σ σ'} : b_deriv (b,σ) false -> c_deriv (c1,σ) σ' -> c_deriv (Com.Ite b c0 c1, σ) σ'
@@ -60,3 +62,95 @@ example : c_equiv (Com.While b c) (Com.Ite b (Com.Seq c (Com.While b c)) Com.Ski
     | ite_true bd cd =>
       cases cd with
       | seq cd0 cd1 => exact c_deriv.while_true bd cd0 cd1
+
+/-! # 3.3 Well-founded induction -/
+
+/- Theorem 3.10 -/
+
+/- euclid := while ¬(M=N) do if M < N then N:=N-M else M:=M-N -/
+def euclid : Com :=
+  Com.While
+    (Bexp.Not (Bexp.Eq (Aexp.Loc "M") (Aexp.Loc "N")))
+    (Com.Ite
+      (Bexp.Le (Aexp.Loc "M") (Aexp.Loc "N"))
+      (Com.Assign "N" (Aexp.Sub (Aexp.Loc "N") (Aexp.Loc "M")))
+      (Com.Assign "M" (Aexp.Sub (Aexp.Loc "M") (Aexp.Loc "N")))
+    )
+
+-- fixme : to simplify a lot
+theorem euclid_deriv :
+    ∀ (σ : State) ,
+    σ{"M"} >= 1 ∧ σ{"N"} >= 1
+    -> ∃ (σ' : State) , c_deriv (euclid,σ) σ'
+:= by
+  intro σ h
+
+  let M := "M"
+  let N := "N"
+  let m := σ{M}
+  let n := σ{N}
+
+  let MsubN := Aexp.Sub (Aexp.Loc M) (Aexp.Loc N)
+  let NsubM := Aexp.Sub (Aexp.Loc N) (Aexp.Loc M)
+  let MeqN := Bexp.Eq (Aexp.Loc M) (Aexp.Loc N)
+  let MleN := Bexp.Le (Aexp.Loc M) (Aexp.Loc N)
+
+  let heq := m = n
+  by_cases heq
+  . have ev := b_eval_deriv (Bexp.Not MeqN) σ
+    have h1 : (m == n) = true := by grind
+    simp [b_eval,a_eval,m,n,h1,MeqN] at ev
+    use σ
+    exact .while_false ev
+  . have ev := b_eval_deriv (Bexp.Not MeqN) σ
+    have h1 : (m == n) = false := by grind
+    simp [b_eval,a_eval,m,n,h1,MeqN] at ev
+    let hlt := m <= n
+    by_cases hlt
+    . have h2 : (m <= n) = true := by grind
+      let σ'' := (N,n-m)::σ
+      have c1 : c_deriv (
+        (Com.Assign N NsubM), σ) σ'' := by
+          apply c_deriv.assign
+          apply a_eval_deriv
+      have c : c_deriv (Com.Ite
+        MleN
+        (Com.Assign N NsubM)
+        (Com.Assign M MsubN), σ) σ'' := by
+          apply c_deriv.ite_true
+          have hhh : (b_eval MleN σ) = true := by rw [b_eval,a_eval,a_eval]; grind
+          have lll := b_eval_deriv MleN σ
+          simp [hhh] at lll
+          trivial
+          exact c1
+      have q1 : σ''{M} = m := by rw [State.lookup]; grind
+      have q2 : σ''{N} = n-m := by rw [State.lookup]; grind
+      have q : σ''{M} >= 1 ∧ σ''{N} >= 1 := by grind
+      have t : ((N, n-m) :: σ){N} < n := by grind
+      have ⟨σ',p⟩ := euclid_deriv σ'' q
+      use σ'
+      exact .while_true ev c p
+    . have h2 : (m <= n) = false := by grind
+      let σ'' := (M,m-n)::σ
+      have c1 : c_deriv (
+        (Com.Assign M MsubN), σ) σ'' := by
+          apply c_deriv.assign
+          apply a_eval_deriv
+      have c : c_deriv (Com.Ite
+        MleN
+        (Com.Assign N NsubM)
+        (Com.Assign M MsubN), σ) σ'' := by
+          apply c_deriv.ite_false
+          have hhh : (b_eval MleN σ) = false := by rw [b_eval,a_eval,a_eval]; grind
+          have lll := b_eval_deriv MleN σ
+          simp [hhh] at lll
+          trivial
+          exact c1
+      have q1 : σ''{M} = m-n := by rw [State.lookup]; grind
+      have q2 : σ''{N} = n := by rw [State.lookup]; grind
+      have q : σ''{M} >= 1 ∧ (σ''{N}) >= 1 := by grind
+      have t : ((M, m-n) :: σ){M} < m := by grind
+      have ⟨σ',p⟩ := euclid_deriv σ'' q
+      use σ'
+      exact .while_true ev c p
+  termination_by σ => (σ{"M"} , σ{"N"})
