DenotationalLean/Imp.lean
@@ -20,7 +20,7 @@ inductive Bexp : Type where
 
 inductive Com : Type where
   | Skip : Com
-  | Assing : Loc -> Aexp -> Com
+  | Assign : Loc -> Aexp -> Com
   | Seq : Com -> Com -> Com
   | Ite : Bexp -> Com -> Com -> Com
   | While : Bexp -> Com -> Com
