DenotationalLean/State.lean
@@ -10,3 +10,5 @@ def lookup(σ : State) : Loc -> Nat := fun l => match σ with
   | ((l',n)::xs) => if l == l' then n else lookup xs l
 
 end State
+
+notation:70 σ:70 "{" l:70 "}" => State.lookup σ l
